Gentlemen, we have work to do.

thy/Abstract_Impl.thy
@@ -6,7 +6,7 @@ begin
 datatype ('a, 'ni) IFEXD = TD | FD | IFD 'a 'ni 'ni 
 
 locale bdd_impl = 
-  fixes R :: "'s \<Rightarrow> ('ni \<times> 'a ifex) set"
+  fixes R :: "'s \<Rightarrow> ('ni \<times> ('a :: linorder) ifex) set"
   fixes Timpl :: "'s \<Rightarrow> ('ni \<times> 's)"
   fixes Fimpl :: "'s \<Rightarrow> ('ni \<times> 's)"
   fixes IFimpl :: "'a \<Rightarrow> 'ni \<Rightarrow> 'ni \<Rightarrow> 's \<Rightarrow> ('ni \<times> 's)"
@@ -48,7 +48,7 @@ partial_function(option) restrict_impl_opt where
                                                         (re,s) \<leftarrow> restrict_impl_opt e var val s;
                                                      if v = var then (if val then Some (rt,s) else Some (re, s)) else
                                                      Some (IFimpl v rt re s)}) |
-                                     i \<Rightarrow> Some (n,s))"
+                                     _ \<Rightarrow> Some (n,s))"
 
 lemma les_refl[simp,intro!]:"les s s" by (auto simp add: les_def)
 lemma les_trans[trans]:"les s1 s2 \<Longrightarrow> les s2 s3 \<Longrightarrow> les s1 s3" by (auto simp add: les_def)
@@ -67,10 +67,52 @@ proof(induction n arbitrary: ni s)
 	from this(3) rnits(2) have 1: "(rnit, restrict n1 var val) \<in> R s''" unfolding les_def by simp
 	obtain r s''' where rs: "IFimpl x1 rnit rnie s'' = (r,s''')" by force
 	have les: "les s s''" "les s s'''" using les_trans rnits(3) rnies(3) IFimpl_mono[OF 1 rnies(2) rs] by blast+
-	show ?case find_theorems "DESTRimpl"
+	show ?case
 		using 1 rnies(2) les IFimpl_rule[OF 1 rnies(2) rs]
 		by(subst restrict_impl_opt.simps, auto simp add: rnits(1) rnies(1) dimp rs)
 qed (force dest: DESTRimpl_rule1 DESTRimpl_rule2 simp add: restrict_impl_opt.simps)+
+
+fun lowest_tops_impl where
+"lowest_tops_impl [] s = None" |
+"lowest_tops_impl (e#es) s = 
+	(case DESTRimpl e s of
+		(IFD v t e) \<Rightarrow> (case lowest_tops_impl es s of 
+			Some u \<Rightarrow> Some (min u v) | 
+			None \<Rightarrow> Some v) |
+		_           \<Rightarrow> lowest_tops_impl es s)"
+fun in_R_list where
+"in_R_list nis [] _ = (case nis of (_#_) \<Rightarrow> False | _ \<Rightarrow> True)" |
+"in_R_list nis (n#ns) s = (case nis of (ni#nis) \<Rightarrow> ((ni, n) \<in> R s) | _ \<Rightarrow> False)"
+
+lemma "in_R_list nis ns s \<Longrightarrow> lowest_tops_impl nis s = lowest_tops ns"
+apply(induction rule: lowest_tops.induct)
+apply(simp split: list.splits)
+defer
+apply(simp split: list.splits)
+oops (* todo *)
+
+(* todo: write restrict_top and use it! (also, that doesn't return state) *)
+partial_function(option) ite_impl where
+"ite_impl i t e s = 
+	(case lowest_tops_impl [i, t, e] s of
+		Some a \<Rightarrow> (do {
+			(ti,s) \<leftarrow> restrict_impl_opt i a True s;
+			(tt,s) \<leftarrow> restrict_impl_opt t a True s;
+			(te,s) \<leftarrow> restrict_impl_opt e a True s;
+			(tb,s) \<leftarrow> ite_impl ti tt te s;
+			(fi,s) \<leftarrow> restrict_impl_opt i a False s;
+			(ft,s) \<leftarrow> restrict_impl_opt t a False s;
+			(fe,s) \<leftarrow> restrict_impl_opt e a False s;
+			(fb,s) \<leftarrow> ite_impl fi ft fe s;
+            Some (IFimpl a tb fb s)}) |
+        None \<Rightarrow> Some undefined)"
+lemma "
+	(ii, i) \<in> R s \<Longrightarrow>
+	(ti, t) \<in> R s \<Longrightarrow>
+	(ei, e) \<in> R s \<Longrightarrow>
+	ite_impl ii ti ei s = Some (r, s') \<Longrightarrow>
+	(r, ifex_ite i t e) \<in> R s'"
+oops (* we have work to do *)
 
 end
 end
